theories/RTL/Rules/Hoare.v
@@ -6,11 +6,11 @@ From RSL.Logic Require Export Logic.
 Import RTLNotations.
 
 Definition hoare {J I} Pt Ps C Pre ft j i fs Post : rProp :=
-  □ (∀ valt vals Ψ,
+  □ (∀ valt vals,
        Pre valt vals -∗
-       (∀ vt vs, Post vt vs -∗ Ψ vt vs) -∗
+       (* (∀ vt vs, Post vt vs -∗ Ψ vt vs) -∗ *)
        @sim_lfp rtl_lang rtl_lang J I Pt Ps C
-         ([], CallState ft valt) j i ([], CallState fs vals) Ψ
+         ([], CallState ft valt) j i ([], CallState fs vals) Post
     )%I.
 
 Notation
@@ -27,25 +27,40 @@ Section HoareRules.
 
   Context {ft : rtl_function} {j: J} {i: I} {fs : rtl_function}.
 
-  Lemma frame F P Q:
-    [Pt, Ps, C] {{ P }} ft <{j, i}= fs {{ Q }} -∗
-    [Pt, Ps, C] {{ fun valt vals => P valt vals ∗ F }} ft <{j, i}= fs {{ fun vt vs => Q vt vs ∗ F }}.
-  Proof using Type.
-    iIntros "#H !>" (valt vals Ψ) "[Hpre Hf] Hpost".
-    iApply ("H" with "Hpre").
-    iIntros (vt vs) "Hq". iApply "Hpost".
-    by iFrame.
-  Qed.
+  (* Lemma frame F P Q: *)
+  (*   [Pt, Ps, C] {{ P }} ft <{j, i}= fs {{ Q }} -∗ *)
+  (*   [Pt, Ps, C] {{ fun valt vals => P valt vals ∗ F }} ft <{j, i}= fs {{ fun vt vs => Q vt vs ∗ F }}. *)
+  (* Proof using Type. *)
+  (*   unfold hoare. unseal. *)
+  (*   intros ? ? [-> ->] mt ms _ _ [[-> ->] Hsim]. smap. *)
+  (*   split. { by split. } *)
+  (*   intros valt vals. *)
+  (*   intros a b _ _ Hpre. smap. *)
+  (*   destruct Hpre as (mtP & msP & mtF & msF & Ht & Hs & <- & <- & HP & HF). simpl. *)
+  (*   apply Hsim in HP; try apply map_disjoint_empty_r. clear Hsim. *)
+  (*   revert mtP msP mtF msF HF Ht Hs HP. simpl. *)
+  (*   apply tower. *)
+  (*   { admit. } *)
+  (*   clear C. intros C CIH. *)
+  (*   intros mtP msP mtF msF HF Ht Hs Hsim. *)
+  (*   induction Hsim. *)
+  (*   - apply FRelated.  *)
+  (*   simpl. *)
+  (*   iIntros "#H !>" (valt vals Ψ) "[Hpre Hf] Hpost". *)
+  (*   iApply ("H" with "Hpre"). *)
+  (*   iIntros (vt vs) "Hq". iApply "Hpost". *)
+  (*   by iFrame. *)
+  (* Qed. *)
 
-  Lemma consequence P P' Q Q':
-    □ (∀ valt vals, P valt vals -∗ P' valt vals) -∗
-    □ (∀ vt vs, Q' vt vs -∗ Q vt vs) -∗
-    [Pt, Ps, C] {{ P' }} ft <{j, i}= fs {{ Q' }} -∗
-    [Pt, Ps, C] {{ P }} ft <{j, i}= fs {{ Q }}.
-  Proof using Type.
-    iIntros "#HP #HQ #H !>" (valt vals Ψ) "Hpre Hpost".
-    iApply ("H" with "[Hpre] [Hpost]").
-    - by iApply "HP".
-    - iIntros (vt vs) "HQ'". iApply "Hpost". by iApply "HQ".
-  Qed.
+  (* Lemma consequence P P' Q Q': *)
+  (*   □ (∀ valt vals, P valt vals -∗ P' valt vals) -∗ *)
+  (*   □ (∀ vt vs, Q' vt vs -∗ Q vt vs) -∗ *)
+  (*   [Pt, Ps, C] {{ P' }} ft <{j, i}= fs {{ Q' }} -∗ *)
+  (*   [Pt, Ps, C] {{ P }} ft <{j, i}= fs {{ Q }}. *)
+  (* Proof using Type. *)
+  (*   iIntros "#HP #HQ #H !>" (valt vals Ψ) "Hpre Hpost". *)
+  (*   iApply ("H" with "[Hpre] [Hpost]"). *)
+  (*   - by iApply "HP". *)
+  (*   - iIntros (vt vs) "HQ'". iApply "Hpost". by iApply "HQ". *)
+  (* Qed. *)
 End HoareRules.
