theories/RTL/Rules/SourceRules.v
@@ -30,44 +30,44 @@ Section SourceRulesDef.
   Context {Pt : prog Λt} {Ps : prog Λs}.
   Context {C : Chain (fsim_lfp WfNat WfNat Pt Ps)}.
 
-  Context (st : pstate Λt) (j i : WfNat) (cs : list stackframe)
+  Context (st : istate Λt) (j i : WfNat) (σs : list stackframe)
     (fs : rtl_function) (pcs : node) (ρs : regbank)
     (Q : value Λt -> value Λs -> rProp).
 
   Lemma source_nop pc:
     fs@pcs is <<{ nop -> pc }>> ->
-    [Pt, Ps, C] st <{j, 1+i}= (cs, State fs pc ρs) {{ Q }} -∗
-    [Pt, Ps, C] st <{j, i}= (cs, State fs pcs ρs) {{ Q }}.
+    [Pt, Ps, C] st <{j, 1+i}= (σs, State fs pc ρs) {{ Q }} -∗
+    [Pt, Ps, C] st <{j, i}= (σs, State fs pcs ρs) {{ Q }}.
   Proof using Type. by source_step. Qed.
 
   Lemma source_nop_noinc pc:
     fs@pcs is <<{ nop -> pc }>> ->
-    [Pt, Ps, C] st <{j, i}= (cs, State fs pc ρs) {{ Q }} -∗
-    [Pt, Ps, C] st <{j, i}= (cs, State fs pcs ρs) {{ Q }}.
+    [Pt, Ps, C] st <{j, i}= (σs, State fs pc ρs) {{ Q }} -∗
+    [Pt, Ps, C] st <{j, i}= (σs, State fs pcs ρs) {{ Q }}.
   Proof using Type. by source_step. Qed.
 
   Lemma source_ret r v:
     fs@pcs is <<{ ret r }>> ->
     ρs@r ⇒ v ->
-    [Pt, Ps, C] st <{j, 1+i}= (cs, ReturnState v) {{ Q }} -∗
-    [Pt, Ps, C] st <{j, i}= (cs, State fs pcs ρs) {{ Q }}.
+    [Pt, Ps, C] st <{j, 1+i}= (σs, ReturnState v) {{ Q }} -∗
+    [Pt, Ps, C] st <{j, i}= (σs, State fs pcs ρs) {{ Q }}.
   Proof using Type. by source_step. Qed.
 
   Lemma source_op pc dst op regs args v:
     fs@pcs is <<{ dst := @op regs -> pc }>> ->
     ρs @ regs ⇒ args ->
     eval_op op args = Some v ->
-    [Pt, Ps, C] st <{j, 1+i}= (cs, State fs pc (⟦dst ⇐ v⟧ρs)) {{ Q }} -∗
-    [Pt, Ps, C] st <{j, i}= (cs, State fs pcs ρs) {{ Q }}.
+    [Pt, Ps, C] st <{j, 1+i}= (σs, State fs pc (⟦dst ⇐ v⟧ρs)) {{ Q }} -∗
+    [Pt, Ps, C] st <{j, i}= (σs, State fs pcs ρs) {{ Q }}.
   Proof using Type. by source_step. Qed.
 
   Lemma source_load pc dst src l vs:
     fs@pcs is <<{ dst := !src -> pc }>> ->
     ρs @ src ⇒ VPtr l ->
     (l →ₛ vs -∗
-     [Pt, Ps, C] st <{j, 1+i}= (cs, State fs pc (⟦dst ⇐ vs⟧ρs)) {{ Q }}) -∗
+     [Pt, Ps, C] st <{j, 1+i}= (σs, State fs pc (⟦dst ⇐ vs⟧ρs)) {{ Q }}) -∗
     l →ₛ vs -∗
-    [Pt, Ps, C] st <{j, i}= (cs, State fs pcs ρs) {{ Q }}.
+    [Pt, Ps, C] st <{j, i}= (σs, State fs pcs ρs) {{ Q }}.
   Proof using Type.
     intros Hpc Haddr. unseal.
     intros ? ? [-> ->] mtS msS _ _ Hsim. smap.
@@ -86,9 +86,9 @@ Section SourceRulesDef.
     ρs @ dst ⇒ VPtr l ->
     ρs @ src ⇒ v ->
     (l →ₛ v -∗
-     [Pt, Ps, C] st <{j, 1+i}= (cs, State fs pc ρs) {{ Q }}) -∗
+     [Pt, Ps, C] st <{j, 1+i}= (σs, State fs pc ρs) {{ Q }}) -∗
     l →ₛ old -∗
-    [Pt, Ps, C] st <{j, i}= (cs, State fs pcs ρs) {{ Q }}.
+    [Pt, Ps, C] st <{j, i}= (σs, State fs pcs ρs) {{ Q }}.
   Proof using Type.
     intros Hpc Haddr Hsrc. unseal.
     intros ? ? [-> ->] mtS msS _ _ Hsim. smap.
@@ -106,12 +106,12 @@ Section SourceRulesDef.
     - eapply Hsim; smap; by solve_map_disjoint.
   Qed.
 
-  Lemma source_alloc pc dst:
+  Lemma source_alloc pc dst v:
     fs@pcs is <<{ dst := alloc () -> pc }>> ->
     (∀ l,
-       l →ₛ VUndef -∗
-       [Pt, Ps, C] st <{j, 1+i}= (cs, State fs pc (⟦dst ⇐ VPtr l⟧ρs)) {{ Q }}) -∗
-    [Pt, Ps, C] st <{j, i}= (cs, State fs pcs ρs) {{ Q }}.
+       l →ₛ v -∗
+       [Pt, Ps, C] st <{j, 1+i}= (σs, State fs pc (⟦dst ⇐ VPtr l⟧ρs)) {{ Q }}) -∗
+    [Pt, Ps, C] st <{j, i}= (σs, State fs pcs ρs) {{ Q }}.
   Proof using Type.
     intros Hpc. unseal.
     intros ? ? [-> ->] mtS msS _ _ Hsim. smap.
@@ -134,9 +134,9 @@ Section SourceRulesDef.
     fs@pcs is <<{ free src -> pc }>> ->
     ρs @ src ⇒ VPtr l ->
     (freeₛ l -∗
-       [Pt, Ps, C] st <{j, 1+i}= (cs, State fs pc ρs) {{ Q }}) -∗
+       [Pt, Ps, C] st <{j, 1+i}= (σs, State fs pc ρs) {{ Q }}) -∗
     l →ₛ v -∗
-    [Pt, Ps, C] st <{j, i}= (cs, State fs pcs ρs) {{ Q }}.
+    [Pt, Ps, C] st <{j, i}= (σs, State fs pcs ρs) {{ Q }}.
   Proof using Type.
     intros Hpc Hsrc. unseal.
     intros ? ? [-> ->] mtS msS _ _ Hsim. smap.
@@ -159,29 +159,31 @@ Section SourceRulesDef.
   Lemma source_if pcT pcF reg b:
     fs@pcs is <<{ if reg then goto pcT else goto pcF }>> ->
     ρs @ reg ⇒ VBool b ->
-    [Pt, Ps, C] st <{j, 1+i}= (cs, State fs (if b then pcT else pcF) ρs) {{ Q }} -∗
-    [Pt, Ps, C] st <{j, i}= (cs, State fs pcs ρs) {{ Q }}.
+    let pc := if b then pcT else pcF in
+    [Pt, Ps, C] st <{j, 1+i}= (σs, State fs pc ρs) {{ Q }} -∗
+    [Pt, Ps, C] st <{j, i}= (σs, State fs pcs ρs) {{ Q }}.
   Proof using Type. by source_step. Qed.
 
-  Lemma source_call dst sig args pc' fn vals:
+  Lemma source_call dst sig args pc' fn vals ss:
     fs@pcs is <<{ dst := @call sig args -> pc' }>> ->
     find_fun Ps sig = Some fn ->
     ρs@args ⇒ vals ->
-    [Pt, Ps, C] st <{j, 1+i}= (Stackframe dst fs pc' ρs :: cs, CallState fn vals) {{ Q }} -∗
-    [Pt, Ps, C] st <{j, i}= (cs, State fs pcs ρs) {{ Q }}.
+    ss = Stackframe dst fs pc' ρs ->
+    [Pt, Ps, C] st <{j, 1+i}= (ss :: σs, CallState fn vals) {{ Q }} -∗
+    [Pt, Ps, C] st <{j, i}= (σs, State fs pcs ρs) {{ Q }}.
   Proof using Type. by source_step. Qed.
 
   Lemma source_callstate args:
     length args = length (rtl_fn_regs fs) ->
     ρs = init_regs (rtl_fn_regs fs) args ->
     pcs = rtl_fn_entrypoint fs ->
-    [Pt, Ps, C] st <{j, 1+i}= (cs, State fs pcs ρs) {{ Q }} -∗
-    [Pt, Ps, C] st <{j, i}= (cs, CallState fs args) {{ Q }}.
+    [Pt, Ps, C] st <{j, 1+i}= (σs, State fs pcs ρs) {{ Q }} -∗
+    [Pt, Ps, C] st <{j, i}= (σs, CallState fs args) {{ Q }}.
   Proof using Type. by source_step. Qed.
 
   Lemma source_retstate v fn pc dst:
-    [Pt, Ps, C] st <{j, 1+i}= (cs, State fn pc (⟦dst ⇐ v⟧ρs)) {{ Q }} -∗
-    [Pt, Ps, C] st <{j, i}= (Stackframe dst fn pc ρs :: cs, ReturnState v) {{ Q }}.
+    [Pt, Ps, C] st <{j, 1+i}= (σs, State fn pc (⟦dst ⇐ v⟧ρs)) {{ Q }} -∗
+    [Pt, Ps, C] st <{j, i}= (Stackframe dst fn pc ρs :: σs, ReturnState v) {{ Q }}.
   Proof using Type. by source_step. Qed.
 
 End SourceRulesDef.
