Makefile
@@ -14,3 +14,6 @@ clean:
 
 check: build
 	find _build/default/$(SRC_DIR) -name "*.vo" -print0 | xargs -0 rocqchk -R _build/default/$(SRC_DIR) $(PROJECT) -silent -o
+
+report: report/report.tex report/macro.tex
+	latexmk -pdf -cd -outdir=./_build/report/ report/report.tex
